src/promising/Promising.v
@@ -1236,6 +1236,175 @@ Module Machine.
       ss. congr.
   Qed.
 
+  Definition promises_from_mem
+             (tid:Id.t) (mem: Memory.t): Promises.t.
+  Proof.
+    induction mem using list_rev_rect.
+    - exact bot.
+    - destruct x.
+      apply (if tid0 == tid
+             then Promises.set (S (List.length (List.rev mem0))) IHmem
+             else IHmem).
+  Defined.
+
+  Lemma promises_from_mem_nil tid:
+    promises_from_mem tid Memory.empty = bot.
+  Proof.
+    unfold promises_from_mem, list_rev_rect, eq_rect. ss.
+    match goal with
+    | [|- context[match ?c with | eq_refl => _ end]] => destruct c
+    end; ss.
+  Qed.
+
+  Lemma promises_from_mem_snoc tid mem msg:
+    promises_from_mem tid (mem ++ [msg]) =
+    if msg.(Msg.tid) == tid
+    then Promises.set (S (List.length mem)) (promises_from_mem tid mem)
+    else promises_from_mem tid mem.
+  Proof.
+    unfold promises_from_mem at 1, list_rev_rect, eq_rect.
+    match goal with
+    | [|- context[match ?c with | eq_refl => _ end]] => destruct c
+    end; ss.
+    rewrite List.rev_involutive, List.rev_app_distr. ss.
+    destruct msg. s. condtac.
+    - inversion e. subst. rewrite ? List.rev_length.
+      f_equal.
+      unfold promises_from_mem, list_rev_rect, eq_rect.
+      match goal with
+      | [|- context[match ?c with | eq_refl => _ end]] => destruct c
+      end; ss.
+    - unfold promises_from_mem, list_rev_rect, eq_rect.
+      match goal with
+      | [|- context[match ?c with | eq_refl => _ end]] => destruct c
+      end; ss.
+  Qed.
+
+  Lemma promises_from_mem_inv
+        ts tid mem
+        (LOOKUP: Promises.lookup (S ts) (promises_from_mem tid mem)):
+    exists loc val, List.nth_error mem ts = Some (Msg.mk loc val tid).
+  Proof.
+    revert LOOKUP. induction mem using List.rev_ind.
+    { rewrite promises_from_mem_nil, Promises.lookup_bot. ss. }
+    rewrite promises_from_mem_snoc. condtac.
+    { rewrite Promises.set_o. condtac.
+      - inversion e. inversion e0. subst.
+        rewrite List.nth_error_app2; [|lia].
+        rewrite Nat.sub_diag. ss.
+        destruct x. esplits; eauto.
+      - i. exploit IHmem; eauto.  i. des.
+        rewrite List.nth_error_app1; eauto.
+        apply List.nth_error_Some. congr.
+    }
+    i. exploit IHmem; eauto.  i. des.
+    rewrite List.nth_error_app1; eauto.
+    apply List.nth_error_Some. congr.
+  Qed.
+
+  Lemma promises_from_mem_lookup
+        mem ts loc val tid
+        (GET: List.nth_error mem ts = Some (Msg.mk loc val tid)):
+    Promises.lookup (S ts) (promises_from_mem tid mem).
+  Proof.
+    revert GET. induction mem using List.rev_ind.
+    { i. apply List.nth_error_In in GET. inv GET. }
+    rewrite promises_from_mem_snoc. condtac.
+    - rewrite Promises.set_o. condtac.
+      + inversion e. inversion e0. subst.
+        rewrite List.nth_error_app2; [|lia].
+        rewrite Nat.sub_diag. ss.
+      + i. apply IHmem.
+        erewrite <- List.nth_error_app1; eauto.
+        assert (H: ts < List.length (mem0 ++ [x])).
+        { rewrite <- List.nth_error_Some. ii. congr. }
+        rewrite List.app_length in H.
+        rewrite Nat.add_1_r in H. inv H; try lia.
+        exfalso. apply c. ss.
+    - i. apply IHmem.
+      destruct (Nat.eq_dec ts (List.length mem0)) eqn:Heq.
+      + inv Heq. rewrite List.nth_error_app2 in GET; try lia.
+        rewrite Nat.sub_diag in GET. ss. inv GET. ss.
+        exfalso. apply c. ss.
+      + rewrite List.nth_error_app1 in GET; auto.
+        assert (H: ts < List.length (mem0 ++ [x])).
+        { rewrite <- List.nth_error_Some. ii. congr. }
+        rewrite List.app_length in H.
+        rewrite Nat.add_1_r in H. inv H; try lia; congr.
+  Qed.
+
+  Lemma promises_from_mem_spec
+        ts tid mem:
+    Promises.lookup (S ts) (promises_from_mem tid mem) <->
+    exists loc val, List.nth_error mem ts = Some (Msg.mk loc val tid).
+  Proof.
+    induction mem using List.rev_ind.
+    { econs.
+      - rewrite promises_from_mem_nil, Promises.lookup_bot. ss.
+      - i. des. destruct ts; ss.
+    }
+    rewrite promises_from_mem_snoc. econs.
+    - condtac.
+      + inversion e. subst. rewrite Promises.set_o. condtac.
+        * inversion e0. subst. i.
+          rewrite List.nth_error_app2, Nat.sub_diag; [|lia]. ss.
+          destruct x. ss. eauto.
+        * intro Y. apply IHmem in Y. des.
+          esplits; eauto. apply nth_error_app_mon. eauto.
+      + intro Y. apply IHmem in Y. des.
+        esplits; eauto. apply nth_error_app_mon. eauto.
+    - i. des. apply nth_error_snoc_inv in H. des; ss.
+      { condtac; eauto. rewrite Promises.set_o. condtac; eauto. }
+      subst. condtac; ss; [|congr]. rewrite Promises.set_o. condtac; [|congr]. ss.
+  Qed.
+
+  Definition init_with_promises (p:program) (mem:Memory.t): Machine.t :=
+    Machine.mk
+      (IdMap.mapi (fun tid stmts =>
+                     (State.init stmts,
+                      Local.init_with_promises (promises_from_mem tid mem)))
+                  p)
+      mem.
+
+  Lemma pf_init_with_promises
+        p promises
+        (MEM: forall msg (MSG: List.In msg promises), IdMap.find msg.(Msg.tid) p <> None):
+    exists m,
+      <<STEP: rtc (Machine.step ExecUnit.promise_step) (Machine.init p) m>> /\
+      <<TPOOL: IdMap.Equal m.(Machine.tpool) (init_with_promises p promises).(Machine.tpool)>> /\
+      <<MEM: m.(Machine.mem) = promises>>.
+  Proof.
+    revert MEM. induction promises using List.rev_ind; i.
+    { esplits; eauto. ii. s. rewrite IdMap.map_spec, IdMap.mapi_spec.
+      destruct (IdMap.find y p); ss.
+      unfold Local.init, Local.init_with_promises. repeat f_equal.
+      rewrite promises_from_mem_nil. ss.
+    }
+    exploit IHpromises; eauto.
+    { i. apply MEM. apply List.in_app_iff. intuition. }
+    i. des. subst. destruct x.
+    hexploit MEM.
+    { apply List.in_app_iff. right. left. eauto. }
+    match goal with
+    | [|- context[(?f <> None) -> _]] => destruct f eqn:FIND
+    end; ss.
+    intro X. clear X.
+    eexists (Machine.mk _ _). esplits.
+    - etrans; [eauto|]. econs 2; [|refl].
+      econs.
+      + rewrite TPOOL, IdMap.mapi_spec, FIND. ss.
+      + econs; ss.
+      + ss.
+    - s. ii. rewrite IdMap.add_spec. condtac; ss.
+      + inversion e. subst. rewrite IdMap.mapi_spec, FIND. s.
+        unfold Local.init_with_promises. repeat f_equal.
+        rewrite promises_from_mem_snoc. condtac; ss.
+      + rewrite TPOOL, ? IdMap.mapi_spec. destruct (IdMap.find y p); ss.
+        unfold Local.init_with_promises. rewrite promises_from_mem_snoc. s.
+        condtac; ss. congr.
+    - ss.
+  Qed.
+
   Lemma rtc_promise_step_spec
         p m
         (STEP: rtc (step ExecUnit.promise_step) (init p) m):
